Update ReifLam

Auto/Translation/ReifLam.lean
@@ -1,4 +1,5 @@
 import Auto.Translation.Lift
+import Std.Data.List.Lemmas
 
 -- Embedding Simply Typed Lambda Calculus into Dependent Type Theory
 -- Simply Typed Lambda Calculus = HOL (without polymorphism)
@@ -9,6 +10,35 @@ inductive LamSort
 | func : LamSort → LamSort → LamSort
 deriving Inhabited, Hashable, BEq
 
+def LamSort.beq : LamSort → LamSort → Bool
+| .atom m,     .atom n     => m == n
+| .func m₁ n₁, .func m₂ n₂ => LamSort.beq m₁ m₂ && LamSort.beq n₁ n₂
+| _,           _           => false
+
+theorem LamSort.beq_refl (a : LamSort) : (a.beq a) = true := by
+  induction a
+  case atom n => simp [beq]
+  case func s1 s2 => simp [beq]; simp [s1, s2]
+
+theorem LamSort.beq_eq (a b : LamSort) : (a.beq b = true) → a = b := by
+  revert b; induction a
+  case atom m =>
+    intro b; cases b
+    case atom n =>
+      intro HEq; simp [beq] at HEq; simp [HEq]
+    case func => simp [beq]
+  case func m₁ n₁ ihm₁ ihn₁ =>
+    intro b; cases b
+    case atom => simp [beq]
+    case func m₂ n₂ =>
+      simp [beq]; intro hm hn;
+      apply And.intro
+      case left => apply ihm₁; apply hm
+      case right => apply ihn₁; apply hn
+
+theorem LamSort.beq_eq_true_eq (a b : LamSort) : (a.beq b = true) = (a = b) :=
+  propext <| Iff.intro (beq_eq a b) (fun h => by subst h; apply beq_refl)
+
 @[reducible] def LamSort.interp.{u} (val : Nat → Sort u) : LamSort → Sort u
 | .atom n => val n
 | .func dom cod => interp val dom → interp val cod
@@ -16,18 +46,144 @@ deriving Inhabited, Hashable, BEq
 inductive LamTerm
 | atom    : Nat → LamTerm
 | bvar    : Nat → LamTerm
--- Supporting polymorphic `eq`
-| eq      : LamTerm → LamTerm → LamTerm
 | lam     : LamSort → LamTerm → LamTerm
 | app     : LamTerm → LamTerm → LamTerm
+deriving Inhabited, Hashable, BEq
 
+-- Typecheck. `val, lctx ⊢ term : type?`
+-- `val : Nat → LamSort` : Valuation
+-- `List LamSort`        : Local Context
+def LamTerm.check (val : Nat → LamSort) : List LamSort → LamTerm → Option LamSort
+| _,    .atom n  => val n
+| lctx, .bvar n  => lctx.get? n
+| lctx, .lam s t =>
+  match t.check val (s :: lctx) with
+  | .some ty => .some (.func s ty)
+  | .none    => .none
+| lctx, .app fn arg =>
+  match fn.check val lctx, arg.check val lctx with
+  | .some (.func ty₁ ty₂), .some argTy =>
+    if ty₁.beq argTy then .some ty₂ else none
+  | _, _ => .none
+
+-- Judgement. `val, lctx ⊢ term : type?`
+structure LamJudge where
+  lctx   : List LamSort
+  rterm  : LamTerm
+  rTy    : LamSort
+deriving Inhabited, Hashable, BEq
+
+inductive LamWF (val : Nat → LamSort) : LamJudge → Prop
+  | ofAtom
+      {lctx : List LamSort} (n : Nat) :
+    LamWF val ⟨lctx, .atom n, val n⟩
+  | ofBVar
+      {lctx : List LamSort} (n : Fin lctx.length) :
+    LamWF val ⟨lctx, .bvar n, lctx[n]⟩
+  | ofLam
+      {lctx : List LamSort}
+      {argTy : LamSort} (bodyTy : LamSort) {body : LamTerm}
+      (H : LamWF val ⟨argTy :: lctx, body, bodyTy⟩) :
+    LamWF val ⟨lctx, .lam argTy body, .func argTy bodyTy⟩
+  | ofApp
+      {lctx : List LamSort}
+      (argTy : LamSort) {resTy : LamSort}
+      {fn : LamTerm} {arg : LamTerm}
+      (HFn : LamWF val ⟨lctx, fn, .func argTy resTy⟩)
+      (HArg : LamWF val ⟨lctx, arg, argTy⟩) :
+    LamWF val ⟨lctx, .app fn arg, resTy⟩
+
+theorem LamTerm.check_if_wf
+  (val : Nat → LamSort) (lctx : List LamSort) (t : LamTerm) (ty : LamSort) :
+  LamWF val ⟨lctx, t, ty⟩ → t.check val lctx = .some ty := by
+  generalize JudgeEq : { lctx := lctx, rterm := t, rTy := ty : LamJudge} = Judge 
+  intro HWf; revert lctx t ty JudgeEq; induction HWf
+  case ofAtom lctx' n =>
+    intros lctx t ty JudgeEq
+    injection JudgeEq with lctx_eq rterm_eq rty_eq;
+    rw [rterm_eq, rty_eq]; rfl
+  case ofBVar lctx' n =>
+    intros lctx t ty JudgeEq
+    injection JudgeEq with lctx_eq rterm_eq rty_eq;
+    rw [lctx_eq, rterm_eq, rty_eq]; apply List.get?_eq_get
+  case ofLam lctx' argTy bodyTy body H H_ih =>
+    intros lctx t ty JudgeEq
+    injection JudgeEq with lctx_eq rterm_eq rty_eq;
+    rw [lctx_eq, rterm_eq, rty_eq];
+    simp [check]; rw [H_ih]; rfl
+  case ofApp lctx' argTy resTy fn arg HFn HArg HFn_ih HArg_ih =>
+    intros lctx t ty JudgeEq
+    injection JudgeEq with lctx_eq rterm_eq rty_eq;
+    rw [lctx_eq, rterm_eq, rty_eq]
+    simp [check];
+    rw [HFn_ih lctx' fn (LamSort.func argTy resTy)] <;> try rfl;
+    rw [HArg_ih lctx' arg argTy] <;> try rfl;
+    simp [LamSort.beq_refl]
+
+theorem LamTerm.wf_if_check
+  (val : Nat → LamSort) (lctx : List LamSort) (t : LamTerm) (ty : LamSort) :
+  t.check val lctx = .some ty → LamWF val ⟨lctx, t, ty⟩ := by
+  generalize JudgeEq : { lctx := lctx, rterm := t, rTy := ty : LamJudge} = Judge
+  intros HWf; revert lctx ty Judge JudgeEq; induction t
+  case atom a =>
+    intros lctx ty Judge JudgeEq HCheck; rw [← JudgeEq]
+    simp [check] at HCheck; rw [← HCheck]; apply LamWF.ofAtom
+  case bvar n =>
+    intros lctx ty Judge JudgeEq HCheck; rw [← JudgeEq]
+    simp [check] at HCheck; rw [List.get?_eq_some] at HCheck
+    cases HCheck;
+    case intro hLt hEq =>
+      rw [← hEq]; apply LamWF.ofBVar (n := ⟨n, hLt⟩)
+  case lam argTy body IH =>
+    intros lctx ty Judge JudgeEq; rw [← JudgeEq];
+    simp [check];
+    generalize CheckEq : check val (argTy :: lctx) body = cRes
+    cases cRes;
+    case none =>
+      intro HWf; simp at HWf;
+    case some bodyTy =>
+      simp; intro tyEq; rw [← tyEq]
+      apply LamWF.ofLam; apply IH _ _ _ _ CheckEq; rfl
+  case app fn arg IHFn IHarg =>
+    intros lctx ty Judge JudgeEq; rw [← JudgeEq];
+    simp [check]
+    generalize CheckFnEq : check val lctx fn = cFnRes
+    generalize CheckArgEq : check val lctx arg = cArgRes
+    cases cFnRes <;> try (intro HWf; simp at HWf)
+    case some fnTy =>
+      cases cArgRes
+      case none => cases fnTy <;> simp at HWf
+      case some argTy =>
+      cases fnTy <;> simp at HWf
+      case func argTy' resTy' =>
+        cases tyEq : LamSort.beq argTy' argTy
+        case false =>
+          simp [tyEq] at HWf
+        case true =>
+          simp [tyEq] at HWf; rw [← HWf];
+          rw [LamSort.beq_eq_true_eq] at tyEq; rw [tyEq] at CheckFnEq;
+          apply LamWF.ofApp argTy
+          case HFn => apply IHFn _ _ _ _ CheckFnEq; rfl
+          case HArg => apply IHarg _ _ _ _ CheckArgEq; rfl
+     
 -- Valuation
-structure LamVal.{u} where
+structure Lam2DVal.{u} where
   tyVal    : Nat → Type (u + 1)
-  constVal : Nat → (s : LamSort) × LamSort.interp tyVal s
+  constVal : Nat → (α : Type (u + 1)) × α
 
--- Interpretation pair, `(Simply typed lambda calculus term, CIC term)`
-structure LamInterp.{u} where
+/-
+  It seems that we cannot write an interpretation function
+    `interp : Lam2DVal → List ((α : Type (u + 1)) × α) → LamTerm → (α : Type (u + 1)) × α`
+  The main problem is that we cannot manipulate types like inductive types,
+    so we will not be able to compare the types of the two arguments of
+    `LamTerm.eq lhs rhs`, and will not be able to test that the
+    argument type of `f` matches the type of `arg` in `LamTerm.app f arg`
+
+  So, we instead inductively define a well-formedness predicate.
+-/
+
+-- Judgement, `lctx ⊢ rterm ≝ mterm : ty`
+structure Lam2DJudge.{u} where
   -- Local context, list of CIC terms
   lctx    : List ((α : Type (u + 1)) × α)
   -- A term in simply typed lambda calculus
@@ -37,26 +193,18 @@ structure LamInterp.{u} where
   -- The CIC term that `rterm` translates into
   mterm   : ty
 
-inductive WF.{u} (val : LamVal.{u}) : LamInterp.{u} → Prop
-  | ofAtom n
-      {lctx : List ((γ : Type (u + 1)) × γ)} :
+inductive WF.{u} (val : Lam2DVal.{u}) : Lam2DJudge.{u} → Prop
+  | ofAtom
+      {lctx : List ((γ : Type (u + 1)) × γ)}
+      (n : Nat) :
     WF val <|
       let ci := val.constVal n
-      let ty := LamSort.interp val.tyVal ci.fst
-      ⟨lctx, (.atom n), ty, ci.snd⟩
+      ⟨lctx, (.atom n), ci.fst, ci.snd⟩
   | ofBVar
       {lctx : List ((α : Type (u + 1)) × α)}
       (n : Fin lctx.length) :
     WF val <|
       ⟨lctx, .bvar n, lctx[n].fst, lctx[n].snd⟩
-  | ofEq
-      {lctx : List ((γ : Type (u + 1)) × γ)}
-      {hlhs hrhs : LamTerm}
-      (α : Type (u + 1)) (lhs rhs : α)
-      (Hl : WF val ⟨lctx, hlhs, α, lhs⟩)
-      (Hr : WF val ⟨lctx, hrhs, α, rhs⟩) :
-    WF val <|
-      ⟨lctx, .eq hlhs hrhs, Type u, EqLift lhs rhs⟩
   | ofLam
       {lctx : List ((γ : Type (u + 1)) × γ)}
       {hs : LamSort} {ht : LamTerm}
@@ -82,21 +230,59 @@ section Example
 
   -- Original: fun (x : Nat) => Nat.succ x
   -- Lifting to: fun (x : GLift Nat) => Nat.succLift x
-  def interpEx₁.{u} : LamInterp.{u} :=
+  def interpEx₁.{u} : Lam2DJudge.{u} :=
     ⟨[], .lam (.atom 0) (.app (.atom 0) (.bvar 0)),
      GLift.{1, u + 1} Nat → GLift.{1, u + 1} Nat, fun (x : GLift Nat) => Nat.succLift x⟩
   
-  def valuation₁.{u} : LamVal.{u} :=
-    ⟨fun _ => GLift Nat, fun _ => ⟨.func (.atom 0) (.atom 0), Nat.succLift⟩⟩
+  def valuation₁.{u} : Lam2DVal.{u} :=
+    ⟨fun _ => GLift Nat,
+     fun _ => ⟨GLift.{1, u + 1} Nat → GLift.{1, u + 1} Nat, Nat.succLift⟩⟩
 
-  def wf.{u} : WF valuation₁.{u} interpEx₁.{u} := by
+  def wf₁.{u} : WF valuation₁.{u} interpEx₁.{u} := by
     apply WF.ofLam
     intro t
     apply WF.ofApp
     case Hfn =>
       apply WF.ofAtom
     case Harg =>
-      apply (WF.ofBVar (lctx :=[{ fst := GLift Nat, snd := t }]) ⟨0, by simp⟩)
+      apply (WF.ofBVar ⟨0, by simp⟩)
+
+  -- Original: Nat.add 2 3
+  -- Lifting to: GLift.up (Nat.add 2 3)
+  def Nat.addLift.{u} (x y : GLift.{1, u} Nat) :=
+    GLift.up (Nat.add (GLift.down x) (GLift.down y))
+
+  def interpEx₂.{u} : Lam2DJudge.{u} :=
+    ⟨[], .app (.app (.atom 0) (.atom 1)) (.atom 2),
+      GLift.{1, u + 1} Nat, GLift.up (Nat.add 2 3)⟩
+
+  def valuation₂.{u} : Lam2DVal.{u} :=
+    ⟨fun _ => GLift Nat, fun n =>
+      [⟨GLift.{1, u + 1} Nat → GLift.{1, u + 1} Nat → GLift.{1, u + 1} Nat, Nat.addLift⟩,
+       ⟨GLift.{1, u + 1} Nat, GLift.up 2⟩, ⟨GLift.{1, u + 1} Nat, GLift.up 3⟩].getD n ⟨GLift.{1, u + 1} Nat, GLift.up 0⟩⟩
+  
+  def wf₂.{u} : WF valuation₂.{u} interpEx₂.{u} := by
+    apply WF.ofApp (fn := Nat.addLift (GLift.up 2))
+    case Hfn =>
+      apply WF.ofApp <;> apply WF.ofAtom
+    case Harg =>
+      apply WF.ofAtom
+
+  -- Original: @Eq Nat 2 3
+  -- Lifting to: GLift.up (@Eq Nat 2 3)
+  def interpEx₃.{u} : Lam2DJudge.{u} :=
+    ⟨[], .app (.app (.atom 0) (.atom 1)) (.atom 2), Type u, GLift (2 = 3)⟩
+  
+  def valuation₃.{u} : Lam2DVal.{u} :=
+    ⟨fun _ => GLift Nat, fun n =>
+      [⟨GLift.{1, u + 1} Nat → GLift.{1, u + 1} Nat → Type u, @EqLift.{1, u + 1, u} Nat⟩,
+       ⟨GLift.{1, u + 1} Nat, GLift.up 2⟩, ⟨GLift.{1, u + 1} Nat, GLift.up 3⟩].getD n ⟨GLift.{1, u + 1} Nat, GLift.up 0⟩⟩
+
+  def wf₃.{u} : WF valuation₃.{u} interpEx₃.{u} := by
+    apply WF.ofApp (fn := @EqLift.{1, u + 1, u} Nat (GLift.up 2))
+    case Hfn =>
+      apply WF.ofApp <;> apply WF.ofAtom
+    case Harg => apply WF.ofAtom
 
 end Example
 
